# 4.10

## a

none full node

$f(1) = f(0) = 0$

## b

$$
f(N) = \frac{N-2}{N} + \frac{1}{N}\sum_{i=0}^{N-1}{(f(i) - i - 1)}
\quad \quad(N>1)
$$

$\frac{N-2}{N}$ is the average number that root is full note
despite two extreme cases that root is the biggest or the smallest

Apart from root node we assum i left nodes and N - i - 1 right nodes,
so the answer is:
$$
f(N) = \frac{N-2}{N} + f(i) + f(N-i-1)
$$

But we don't know what i is, so we sum of all cases,
from i = 0 through N-1, and then divide them by N to
gain the average number of left subtree and right subtree.

So f(N) is the Sum of the average number of root, left subtree
and right subtree

## c

$$
f(2) = 0 + \frac{1}{2} +
\sum_{i=0}^{1}(f(i)+f(2-i-1)) = 0
$$

So the initial contition is true.

Assume formula is true for N = k (k > 2).

$$
f(k) = \frac{k-2}{k} +
\frac{1}{k}\sum_{i=0}^{k-1}{(f(i) + f(k-i-1))}
= \frac{k-2}{3}
\quad \quad(k>2)
$$

We can gain
$$
\left\{
\begin{align}
    &\sum_{i=0}^{k-1}{(f(i) + f(k-i-1))}
    = \frac{k^2-5k+6}{3}\quad\\
    &f(k) = \frac{k-2}{3}\quad\\
    &f(0) = f(1) = 0\quad

\end{align}
\right.
$$

k+1:
$$
\begin{align*}
    f(k+1) &= \frac{k-1}{k+1} +
    \frac{1}{k+1}\sum_{i=0}^{k}{(f(i)+f(k-i))}\\
    f(k+1) &= \frac{k-1}{k+1} +
    \frac{1}{k+1}\sum_{i=0}^{k-1}{(f(i)+f(k-i))} + f(k) - f(0)\\
    f(k+1) &= \frac{k-1}{k+1} +
    \frac{1}{k+1}\sum_{i=0}^{k-1}{(f(i)+f(k-i))} + f(k)
\end{align*}
$$

We discuss the formula (1):
$$
\begin{align*}
   &\sum_{i=0}^{k-1}{(f(i) + f(k-i-1))}\\
   &= f(0) + f(k-1) + f(1) + f(k-2) + ......
   +f(k-2) + f(1) + f(k-1) + f(0)\\
   &\sum_{i=0}^{k-1}{(f(i) + f(k-i))}\\
   &= f(0) + f(k) + f(1) + f(k-1) + ......
   +f(k-2) + f(2) + f(k-1) + f(1)
\end{align*}
$$

So:
$$
\begin{align*}
   &\sum_{i=0}^{k-1}{(f(i) + f(k-i))}
   -\sum_{i=0}^{k-1}{(f(i) + f(k-i-1))}\\
   &= f(k) - f(0)\\
   &= f(k)\\
   &\sum_{i=0}^{k-1}{(f(i) + f(k-i))}
   = \sum_{i=0}^{k-1}{(f(i) + f(k-i-1))} + f(k)
\end{align*}
$$

So the formula above:
$$
\begin{align*}
    f(k+1) &= \frac{k-1}{k+1} +
    \frac{1}{k+1}\sum_{i=0}^{k-1}{(f(i)-f(k-i))} + f(k)\\
    &= \frac{k-1}{k+1} + \frac{1}{k+1}\times
    (\frac{k^2-5k+6}{3} + \frac{2(k-2)}{3})\\
    &= \frac{k^2-1}{3(k+1)}\\
    &= \frac{k-1}{3}\\
    &= \frac{(k+1) - 2}{3}
\end{align*}
$$

## d

In exercises 4.6, we know that $F + 1 = L$

$$
\begin{align*}
F &= f(N) = \frac{N-2}{3}\\
L &= f(N) + 1 = \frac{N+1}{3}
\end{align*}
$$
